Tests/package.lean
@@ -4,4 +4,4 @@ import «Tests».PrimeRefinementProvider
 import «Tests».PrimeRefinementDemo
 import «Tests».DOT.Sanity
 import «Tests».DTLC.package
-import «Tests».STLC.Scratch
+import «Tests».STLC.package
